src/lowparse/pulse/LowParse.PulseParse.BoundedIntLE.fst
@@ -1,7 +1,6 @@
 module LowParse.PulseParse.BoundedIntLE
 #lang-pulse
 include LowParse.Spec.BoundedInt
-friend LowParse.Spec.BoundedInt
 open Pulse.Lib.Pervasives
 open LowParse.Spec.Combinators
 
